change econv, again

Cedille2/FomegaModel/Soundness.lean
@@ -1,5 +1,6 @@
 
 import Cedille2.Proof
+import Cedille2.Basic
 import Fomega.Basic.Derivations
 import Cedille2.FomegaModel.Interpretation
 
@@ -13,14 +14,51 @@ namespace FomegaModel
   theorem kind_soundness_lemma : Cedille2.Judgment v Γ ix -> KindSoundnessLemmaType v ix := by
   intro j
   induction j <;> simp at *
-  case _ => sorry
-  case _ => sorry
-  case _ => sorry
-  case _ => sorry
-  case _ => sorry
-  case _ => sorry
-  case _ => sorry
-  case _ => sorry
+  case _ => intro Δ wf; constructor; apply wf
+  case _ j1 j2 ih =>
+    intro e Δ wf; subst e; rw [<-j2] at j1
+    exfalso; apply Cedille2.Proof.kind_not_proof j1
+  case _ Γ A m K B j1 j2 ih1 ih2 =>
+    intro e Δ wf
+    cases m <;> simp at *
+    case _ =>
+      split
+      case _ h =>
+        have lem := Cedille2.Proof.classify_kind j1 h
+        injection lem with e; subst e; simp at *
+        have lem1 := ih1 _ wf
+        have lem2 : ⊢ω (𝒱 A :: Δ) := by
+          constructor; apply wf; apply lem1
+        constructor; apply lem1
+        apply ih2 _ lem2
+        constructor
+      case _ h =>
+        cases K <;> simp at *
+        case _ =>
+          have lem := Cedille2.Proof.is_kind_forces_classify j1 rfl
+          exfalso; apply h lem
+        case _ =>
+          have lem2 : ⊢ω (★ :: Δ) := by
+            constructor; apply wf; constructor; apply wf
+          constructor; constructor; apply wf
+          apply ih2 _ lem2
+          constructor
+  case _ j1 j2 j3 ih1 ih2 =>
+    intro e Δ wf; subst e
+    -- by: classification, inversion on `∀(m)[A][B], substitution, □ not a subexpr
+    sorry
+  case _ =>
+    -- by: classification and □ not a subexpr
+    sorry
+  case _ =>
+    -- by: classification and □ not a subexpr
+    sorry
+  case _ j1 j2 j3 ih1 ih2 =>
+    intro h Δ wf; subst h
+    exfalso; apply Cedille2.Proof.kind_not_proof j2
+  case _ j1 j2 j3 ih1 ih1 =>
+    intro h Δ wf; subst h
+    exfalso; apply Cedille2.Proof.kind_not_proof j2
 
   theorem kind_soundness :
     Γ ⊢c t : □ ->
@@ -29,10 +67,61 @@ namespace FomegaModel
   intro j
   apply kind_soundness_lemma j rfl
 
+  @[simp]
+  abbrev TypeSoundnessLemmaType (Γ : Ctx Cedille2.Term) : (v : Cedille2.JudgmentVariant) -> Cedille2.JudgmentIndex v -> Prop
+  | .prf => λ (t, A) => Γ ⊢c A : □ -> γ' Γ ⊢ 𝒯 t : 𝒱 A
+  | .wf => λ _ => True
+
+  theorem type_soundness_lemma : Cedille2.Judgment v Γ ix -> TypeSoundnessLemmaType Γ v ix := by
+  intro j; induction j <;> simp
+  case _ =>
+    intro j; exfalso
+    apply Cedille2.Proof.kind_not_proof j
+  case _ Γ x K T j1 j2 ih =>
+    intro j3; cases K <;> simp at *
+    case _ =>
+
+      sorry
+    case _ =>
+
+      sorry
+  case _ Γ A m K B j1 j2 ih1 ih2 =>
+    intro j3; cases m <;> simp at *
+    case _ =>
+      have lem1 := Cedille2.Proof.is_type_forces_classify j1 j3
+      replace ih1 := ih1 j3
+      replace ih2 := ih2 (Cedille2.Proof.weaken j1 j3)
+      rw [lem1]; rw [lem1] at ih2; simp at *
+      sorry
+    case _ => sorry
+    case _ =>
+      exfalso; apply Cedille2.Proof.kind_not_proof j3
+  case _ => sorry
+  case _ => sorry
+  case _ => sorry
+  case _ =>
+    intro j; cases j
+    case _ j =>
+      exfalso; apply Cedille2.Proof.kind_not_proof j
+  case _ => sorry
+  case _ => sorry
+  case _ => sorry
+  case _ =>
+    intro j; cases j
+    case _ j =>
+      exfalso; apply Cedille2.Proof.kind_not_proof j
+  case _ => sorry
+  case _ =>
+    intro j; cases j
+    case _ j =>
+      exfalso; apply Cedille2.Proof.kind_not_proof j
+  case _ => sorry
+  case _ => sorry
+
   theorem type_soundness :
     Γ ⊢c t : A ->
     Γ ⊢c A : □ ->
-    γ Γ ⊢ 𝒯 t : 𝒱 A
+    γ' Γ ⊢ 𝒯 t : 𝒱 A
   := by sorry
 
   theorem term_soundness :
