Cedille2/Basic.lean
@@ -3,3 +3,5 @@ import Cedille2.Basic.Classification
 import Cedille2.Basic.Substitution
 import Cedille2.Basic.Weaken
 import Cedille2.Basic.Preservation
+import Cedille2.Basic.Inversion
+import Cedille2.Basic.Classify
