Cedille2/FomegaModel/Interpretation.lean
@@ -11,11 +11,9 @@ namespace FomegaModel
   notation:170 Γ:170 " ⊢ω " t:170 " : " A:170 => Fomega.Judgment Fomega.JudgmentVariant.prf Γ (t, A)
   notation:170 "⊢ω " Γ:170 => Fomega.Judgment Fomega.JudgmentVariant.wf Γ ()
 
-  @[simp]
   def drop1 : Fomega.Term -> Fomega.Term -> Fomega.Term
   | d, t => .unit_rec d (u) t
 
-  @[simp]
   def drop2 : Fomega.Term -> Fomega.Term -> Fomega.Term -> Fomega.Term
   | d1, d2, t => drop1 d1 (drop1 d2 t)
 
@@ -24,7 +22,7 @@ namespace FomegaModel
   | □ | ★ => ★
   | .all _ A B =>
     if A.classify = .kind then .all (𝒱 A) (𝒱 B)
-    else 𝒱 B
+    else .all ★ (𝒱 B)
   | _ => □
 
   @[simp]
@@ -36,11 +34,11 @@ namespace FomegaModel
     else Π[★] Π[𝒯 A] 𝒯 B
   | .lam .type A t =>
     if A.classify = .kind then `λ[𝒱 A] 𝒯 t
-    else 𝒯 t
+    else `λ[★] 𝒯 t
   | .app .type f a =>
     if a.classify = .type then (𝒯 f) `@ (𝒯 a)
-    else  𝒯 f
-  | .inter_ty A B => (𝒯 A) ⊗ (𝒯 B)
+    else  (𝒯 f) `@ (U)
+  | .inter_ty A B => (𝒯 A) ⊗ (𝒯 (B β[□]))
   | .eq _ _ => (U)
   | _ => □
 
@@ -48,44 +46,46 @@ namespace FomegaModel
   def γ : Ctx Cedille2.Term -> Ctx Fomega.Term
   | [] => []
   | .cons A Γ =>
-    if A.classify = .kind then (𝒯 A) :: (𝒱 A) :: (γ Γ)
-    else (𝒯 A) :: (𝒯 A) :: (γ Γ)
+    if A.classify = .kind then (𝒱 A) :: (𝒯 A) :: (γ Γ)
+    else ★ :: (𝒯 A) :: (γ Γ)
 
   @[simp]
-  def canon : Cedille2.Term -> Fomega.Term
+  def γ' : Ctx Cedille2.Term -> Ctx Fomega.Term
+  | Γ => Fomega.Term.Bot :: γ Γ
+
+  def canτ : Cedille2.Term -> Fomega.Term
+  | B => #0 `@ 𝒯 B
+
+  def canκ : Cedille2.Term -> Fomega.Term
   | ★ => (U)
-  | .all mf A B =>
-    if B.classify = .kind then `λ[𝒯 A] (canon B)
-    else .unit_rec (𝒯 (.all mf A B)) (u) (u)
-  | B => .unit_rec (𝒯 B) (u) (u)
+  | .all mf A B => `λ[𝒯 A] (canκ B)
+  | _ => □
 
   @[simp]
   def 𝓉 : Cedille2.Term -> Fomega.Term
   | ★ => (u)
-  | .var .type x => #(2*x)
-  | .var .kind x => #(2*x + 1)
-  | .all _ A B => □
-    -- if A.classify = .kind then
-    --   uid2 (𝓉 A) (uid2 ((𝓉 B) β[uid2 (𝒯 A) (u)] β[uid2 (𝒱 A) (u)]) (u))
-    -- else
-    --   c (∀f[zr] ∀f[zr] zr) `@f 𝓉 A `@f (𝓉 B) β[c (𝒯 A)] β[zr]
-  | .lam _ A t => □
-    -- if A.classify = .kind then
-    --   (λf[zr] λf[𝒱 A] λf[𝒯 A] 𝓉 t) `@f 𝓉 A
-    -- else
-    --   (λf[zr] λf[★] λf[𝒯 A] 𝓉 t) `@f 𝓉 A
+  | .var .type x => #(2*x + 1)
+  | .var .kind x => #(2*x + 2)
+  | .all _ A B => (`λ[(U)] `λ[(U)] (u)) `@ (𝓉 A) `@ (𝓉 B β[canκ A] β[canτ A])
+  | .lam _ A t =>
+    if A.classify = .kind then
+      (`λ[(U)] `λ[𝒱 A] `λ[𝒯 A] 𝓉 t) `@ 𝒯 A
+    else
+      (`λ[(U)] `λ[★] `λ[𝒯 A] 𝓉 t) `@ 𝒯 A
   | .app _ f a =>
-    if a.classify = .type then 𝓉 f `@ 𝒯 a `@ 𝓉 a
-    else 𝓉 f `@ (U) `@ 𝓉 a
-  | .inter_ty A B => □
-  | .inter _ _ B t s => □
+    if a.classify = .type then
+      𝓉 f `@ 𝒯 a `@ 𝓉 a
+    else
+      𝓉 f `@ (U) `@ 𝓉 a
+  | .inter_ty A B => (`λ[(U)] `λ[(U)] (u)) `@ (𝓉 A) `@ (𝓉 B)
+  | .inter _ _ B t s => (`λ[(U)] .pair (𝓉 t) (𝓉 s)) `@ (𝓉 B)
   | .fst t => .fst (𝓉 t)
   | .snd t => .snd (𝓉 t)
-  | .eq a b => □
+  | .eq a b => drop2 (𝓉 a) (𝓉 b) (u)
   | .refl t => drop1 (𝓉 t) (u)
-  | .subst Pr e t => □
-  | .phi a b e => □
-  | .conv _ _ A t => □
+  | .subst Pr e t => .unit_rec (𝓉 Pr) (𝓉 e) (𝓉 t)
+  | .phi a b e => .unit_rec (𝓉 a) (𝓉 e) (𝓉 b)
+  | .conv _ _ A t => drop1 (𝓉 A) (𝓉 t)
   | _ => □
 
 end FomegaModel
